src/Std/Data/DTreeMap/Raw/Slice.lean
@@ -18,15 +18,17 @@ public instance {α : Type u} {β : α → Type v}
     Rii.Sliceable (Raw α β cmp) α (Internal.RiiSlice α β) where
   mkSlice carrier range := ⟨carrier.inner, range⟩
 
-public theorem toList_rii {α : Type u} {β : α → Type v} [Ord α] {t : Raw α β compare} : t[*...*].toList = t.toList := by
+@[simp] public theorem toList_rii {α : Type u} {β : α → Type v}
+    [Ord α] {t : Raw α β compare} : t[*...*].toList = t.toList := by
   apply Internal.toList_rii
 
 public instance {α : Type u} {β : α → Type v} [Ord α] (cmp : α → α → Ordering := by exact compare) :
     Ric.Sliceable (Raw α β cmp) α (Internal.RicSlice α β) where
   mkSlice carrier range := ⟨carrier.inner, range⟩
 
-public theorem toList_ric {α : Type u} {β : α → Type v} [Ord α] [TransOrd α] {t : Raw α β compare} {wf : t.WF} {bound : α} :
-  t[*...=bound].toList = t.toList.filter (fun e => (compare e.fst bound).isLE) := by
+public theorem toList_ric {α : Type u} {β : α → Type v} [Ord α] [TransOrd α]
+    {t : Raw α β compare} {wf : t.WF} {bound : α} :
+    t[*...=bound].toList = t.toList.filter (fun e => (compare e.fst bound).isLE) := by
   apply Internal.toList_ric
   . exact wf.out.ordered
 
@@ -35,7 +37,7 @@ public instance {α : Type u} {β : α → Type v} [Ord α] (cmp : α → α →
   mkSlice carrier range := ⟨carrier.inner, range⟩
 
 public theorem toList_rio {α : Type u} {β : α → Type v} [Ord α] [TransOrd α] {t : Raw α β compare} {wf : t.WF} {bound : α} :
-  t[*...<bound].toList = t.toList.filter (fun e => (compare e.fst bound).isLT) := by
+    t[*...<bound].toList = t.toList.filter (fun e => (compare e.fst bound).isLT) := by
   apply Internal.toList_rio
   . exact wf.out.ordered
 
@@ -44,7 +46,7 @@ public instance {α : Type u} {β : α → Type v} [Ord α] (cmp : α → α →
   mkSlice carrier range := ⟨carrier.inner, range⟩
 
 public theorem toList_rci {α : Type u} {β : α → Type v} [Ord α] [TransOrd α] {t : Raw α β compare} {wf : t.WF} {bound : α} :
-  t[bound...*].toList = t.toList.filter (fun e => (compare e.fst bound).isGE) := by
+    t[bound...*].toList = t.toList.filter (fun e => (compare e.fst bound).isGE) := by
   apply Internal.toList_rci
   . exact wf.out.ordered
 
@@ -52,8 +54,9 @@ public instance {α : Type u} {β : α → Type v} [Ord α] (cmp : α → α →
     Rco.Sliceable (Raw α β cmp) α (Internal.RcoSlice α β) where
   mkSlice carrier range := ⟨carrier.inner, range⟩
 
-public theorem toList_rco {α : Type u} {β : α → Type v} [Ord α] [TransOrd α] {t : Raw α β compare} {wf : t.WF} {lowerBound upperBound : α} :
-  t[lowerBound...<upperBound].toList = t.toList.filter (fun e => (compare e.fst lowerBound).isGE ∧ (compare e.fst upperBound).isLT) := by
+public theorem toList_rco {α : Type u} {β : α → Type v} [Ord α] [TransOrd α] {t : Raw α β compare}
+    {wf : t.WF} {lowerBound upperBound : α} : t[lowerBound...<upperBound].toList =
+      t.toList.filter (fun e => (compare e.fst lowerBound).isGE ∧ (compare e.fst upperBound).isLT) := by
   apply Internal.toList_rco
   . exact wf.out.ordered
 
@@ -61,9 +64,9 @@ public instance {α : Type u} {β : α → Type v} [Ord α] (cmp : α → α →
     Rcc.Sliceable (Raw α β cmp) α (Internal.RccSlice α β) where
   mkSlice carrier range := ⟨carrier.inner, range⟩
 
-public theorem toList_rcc {α : Type u} {β : α → Type v} [Ord α] [TransOrd α] {t : Raw α β compare} {wf : t.WF} {lowerBound upperBound : α} :
-  t[lowerBound...=upperBound].toList =
-    t.toList.filter (fun e => (compare e.fst lowerBound).isGE ∧ (compare e.fst upperBound).isLE) := by
+public theorem toList_rcc {α : Type u} {β : α → Type v} [Ord α] [TransOrd α] {t : Raw α β compare}
+    {wf : t.WF} {lowerBound upperBound : α} : t[lowerBound...=upperBound].toList =
+      t.toList.filter (fun e => (compare e.fst lowerBound).isGE ∧ (compare e.fst upperBound).isLE) := by
   apply Internal.toList_rcc
   . exact wf.out.ordered
 
@@ -71,9 +74,9 @@ public instance {α : Type u} {β : α → Type v} [Ord α] (cmp : α → α →
     Roi.Sliceable (Raw α β cmp) α (Internal.RoiSlice α β) where
   mkSlice carrier range := ⟨carrier.inner, range⟩
 
-public theorem toList_roi {α : Type u} {β : α → Type v} [Ord α] [TransOrd α] {t : Raw α β compare} {wf : t.WF} {bound: α} :
-  t[bound<...*].toList =
-    t.toList.filter (fun e => (compare e.fst bound).isGT) := by
+public theorem toList_roi {α : Type u} {β : α → Type v} [Ord α] [TransOrd α]
+    {t : Raw α β compare} {wf : t.WF} {bound: α} : t[bound<...*].toList =
+      t.toList.filter (fun e => (compare e.fst bound).isGT) := by
   apply Internal.toList_roi
   . exact wf.out.ordered
 
@@ -81,9 +84,9 @@ public instance {α : Type u} {β : α → Type v} [Ord α] (cmp : α → α →
     Roc.Sliceable (Raw α β cmp) α (Internal.RocSlice α β) where
   mkSlice carrier range := ⟨carrier.inner, range⟩
 
-public theorem toList_roc {α : Type u} {β : α → Type v} [Ord α] [TransOrd α] {t : Raw α β compare} {wf : t.WF} {lowerBound upperBound : α} :
-  t[lowerBound<...=upperBound].toList =
-    t.toList.filter (fun e => (compare e.fst lowerBound).isGT ∧ (compare e.fst upperBound).isLE) := by
+public theorem toList_roc {α : Type u} {β : α → Type v} [Ord α] [TransOrd α] {t : Raw α β compare}
+    {wf : t.WF} {lowerBound upperBound : α} : t[lowerBound<...=upperBound].toList =
+      t.toList.filter (fun e => (compare e.fst lowerBound).isGT ∧ (compare e.fst upperBound).isLE) := by
   apply Internal.toList_roc
   . exact wf.out.ordered
 
@@ -91,9 +94,9 @@ public instance {α : Type u} {β : α → Type v} [Ord α] (cmp : α → α →
     Roo.Sliceable (Raw α β cmp) α (Internal.RooSlice α β) where
   mkSlice carrier range := ⟨carrier.inner, range⟩
 
-public theorem toList_roo {α : Type u} {β : α → Type v} [Ord α] [TransOrd α] {t : Raw α β compare} {wf : t.WF} {lowerBound upperBound : α} :
-  t[lowerBound<...upperBound].toList =
-    t.toList.filter (fun e => (compare e.fst lowerBound).isGT ∧ (compare e.fst upperBound).isLT) := by
+public theorem toList_roo {α : Type u} {β : α → Type v} [Ord α] [TransOrd α]
+    {t : Raw α β compare} {wf : t.WF} {lowerBound upperBound : α} : t[lowerBound<...upperBound].toList =
+      t.toList.filter (fun e => (compare e.fst lowerBound).isGT ∧ (compare e.fst upperBound).isLT) := by
   apply Internal.toList_roo
   . exact wf.out.ordered
 
